Refactored Cert and Signature modules, updated tests

src/tls/Cert.fst
@@ -6,12 +6,11 @@ open Platform.Error
 open TLSError
 open TLSConstants
 open CoreCrypto
-open Signature
 
-type hint = string
 type cert = b:bytes {length b <= 16777215}
 type chain = list cert
 
+(* ------------------------------------------------------------------------ *)
 abstract val certificateListBytes: chain -> Tot bytes
 let rec certificateListBytes l =
   match l with
@@ -21,261 +20,104 @@ let rec certificateListBytes l =
     (vlbytes 3 c) @| (certificateListBytes r)
 
 val certificateListBytes_is_injective: c1:chain -> c2:chain ->
-  Lemma (requires (True))
-	(ensures (Seq.equal (certificateListBytes c1) (certificateListBytes c2) ==> c1 = c2))
+  Lemma (Seq.equal (certificateListBytes c1) (certificateListBytes c2) ==> c1 = c2)
 let rec certificateListBytes_is_injective c1 c2 =
   match c1, c2 with
   | [], [] -> ()
   | hd::tl, hd'::tl' ->
-      if certificateListBytes c1 = certificateListBytes c2 then (
-	lemma_repr_bytes_values (length hd); lemma_repr_bytes_values (length hd');
-	cut(Seq.equal ((vlbytes 3 hd) @| (certificateListBytes tl)) ((vlbytes 3 hd') @| (certificateListBytes tl')));
-	lemma_repr_bytes_values (length hd);
-	lemma_repr_bytes_values (length hd');	
-	cut(Seq.equal (Seq.slice (vlbytes 3 hd) 0 3) (Seq.slice (certificateListBytes c1) 0 3));
-	cut(Seq.equal (Seq.slice (vlbytes 3 hd') 0 3) (Seq.slice (certificateListBytes c1) 0 3));
-	vlbytes_length_lemma 3 hd hd';
-	lemma_append_inj (vlbytes 3 hd) (certificateListBytes tl) (vlbytes 3 hd') (certificateListBytes tl');
-	lemma_vlbytes_inj 3 hd hd';
-	certificateListBytes_is_injective tl tl';
-	()
-      )
-  | [], hd::tl -> (
-      cut (length (certificateListBytes c1) = 0); 
+    if certificateListBytes c1 = certificateListBytes c2 then
+      begin
+      lemma_repr_bytes_values (length hd); lemma_repr_bytes_values (length hd');
+      cut(Seq.equal ((vlbytes 3 hd) @| (certificateListBytes tl)) ((vlbytes 3 hd') @| (certificateListBytes tl')));
       lemma_repr_bytes_values (length hd);
-      cut (Seq.equal (certificateListBytes c2) ((vlbytes 3 hd) @| (certificateListBytes tl)));
-      lemma_vlbytes_len 3 hd
-    )
-  | hd::tl, [] -> (
-      cut (length (certificateListBytes c2) = 0); 
-      lemma_repr_bytes_values (length hd);
-      cut (Seq.equal (certificateListBytes c1) ((vlbytes 3 hd) @| (certificateListBytes tl)));
-      lemma_vlbytes_len 3 hd
-  )
-	
+      lemma_repr_bytes_values (length hd');
+      cut(Seq.equal (Seq.slice (vlbytes 3 hd) 0 3) (Seq.slice (certificateListBytes c1) 0 3));
+      cut(Seq.equal (Seq.slice (vlbytes 3 hd') 0 3) (Seq.slice (certificateListBytes c1) 0 3));
+      vlbytes_length_lemma 3 hd hd';
+      lemma_append_inj (vlbytes 3 hd) (certificateListBytes tl) (vlbytes 3 hd') (certificateListBytes tl');
+      lemma_vlbytes_inj 3 hd hd';
+      certificateListBytes_is_injective tl tl'
+      end
+  | [], hd::tl ->
+    begin
+    cut (length (certificateListBytes c1) = 0);
+    lemma_repr_bytes_values (length hd);
+    cut (Seq.equal (certificateListBytes c2) ((vlbytes 3 hd) @| (certificateListBytes tl)));
+    lemma_vlbytes_len 3 hd
+    end
+  | hd::tl, [] ->
+    begin
+    cut (length (certificateListBytes c2) = 0);
+    lemma_repr_bytes_values (length hd);
+    cut (Seq.equal (certificateListBytes c1) ((vlbytes 3 hd) @| (certificateListBytes tl)));
+    lemma_vlbytes_len 3 hd
+    end
+
 abstract val parseCertificateList: b:bytes -> Tot (result chain) (decreases (length b))
 let rec parseCertificateList b =
   if length b >= 3 then
     match vlsplit 3 b with
     | Correct (c,r) ->
-	cut (repr_bytes (length c) <= 3);
-        let rl = parseCertificateList r in
-        (match rl with
-        | Correct x -> (
-	    lemma_repr_bytes_values (length c);
-	    Correct (c::x)
-	    )
-        | e -> e)
+      cut (repr_bytes (length c) <= 3);
+      let rl = parseCertificateList r in
+      begin
+      match rl with
+      | Correct x -> (lemma_repr_bytes_values (length c); Correct (c::x))
+      | e -> e
+      end
     | _ -> Error(AD_bad_certificate_fatal, perror __SOURCE_FILE__ __LINE__ "Badly encoded certificate list")
   else if length b = 0 then Correct []
   else Error(AD_bad_certificate_fatal, perror __SOURCE_FILE__ __LINE__ "Badly encoded certificate list")
 
 val lemma_parseCertificateList_length: b:bytes -> 
-  Lemma (requires (True))
-	(ensures (match parseCertificateList b with
+  Lemma (ensures (match parseCertificateList b with
 		  | Correct ces -> length (certificateListBytes ces) = length b
 		  | _ -> True))
 	(decreases (length b))
 let rec lemma_parseCertificateList_length b = 
   match parseCertificateList b with
-  | Correct([]) -> ()
-  | Correct (hd::tl) -> begin
-      cut(length b >= 3);
-      match vlsplit 3 b with
-      | Correct (c, r) ->
-	  lemma_parseCertificateList_length r;
-	  ()
-      | _ -> ()
+  | Correct [] -> ()
+  | Correct (hd::tl) ->
+    begin
+    cut(length b >= 3);
+    match vlsplit 3 b with
+    | Correct (c, r) -> lemma_parseCertificateList_length r
+    | _ -> ()
     end
   | Error _ -> ()
 
+
+(* ------------------------------------------------------------------------ *)
 (* JK: why is that necessary ? *)
 (* SZ: proving that `chain` is a subtype of `list bytes` requires a positivity check *)
-let rec list_chain_is_list_bytes (c:chain) : Tot (list bytes) = 
+private let rec list_chain_is_list_bytes (c:chain) : Tot (list bytes) =
   match c with
   | [] -> []
   | hd::tl -> hd::(list_chain_is_list_bytes tl)
 
-val validate_chain : chain -> option sigAlg -> option string -> string -> Tot bool
-let validate_chain c sigalg host cafile =
-  let for_signing = match sigalg with | None -> false | _ -> true in
+val validate_chain: chain -> bool -> option string -> string -> Tot bool
+let validate_chain c for_signing host cafile =
   let c = list_chain_is_list_bytes c in
   CoreCrypto.validate_chain c for_signing host cafile
 
-val get_chain_public_signing_key : chain -> sigAlg -> Tot (result Signature.public_repr)
-let get_chain_public_signing_key c a =
-  match c with
-  | cert::_ -> (
-    (* let cert = List.Tot.hd c in *)
-    match a with
-    | DSA ->
-      begin
-      match CoreCrypto.get_dsa_from_cert cert with
-      | None -> Error(AD_internal_error, perror __SOURCE_FILE__ __LINE__ "failed to get signing key")
-      | Some k -> Correct (PK_DSA k)
-      end
-      | RSASIG ->
-      begin
-      match CoreCrypto.get_rsa_from_cert cert with
-      | None -> Error(AD_internal_error, perror __SOURCE_FILE__ __LINE__ "failed to get signing key")
-      | Some k -> Correct (PK_RSA k)
-      end
-      | ECDSA ->
-      begin
-      match CoreCrypto.get_ecdsa_from_cert cert with
-      | None -> Error(AD_internal_error, perror __SOURCE_FILE__ __LINE__ "failed to get signing key")
-      | Some k -> Correct (PK_ECDSA k)
-      end
-      | RSAPSS ->
-    Error(AD_internal_error, perror __SOURCE_FILE__ __LINE__ "unimplemented") )
-  | _ -> Error(AD_internal_error, perror __SOURCE_FILE__ __LINE__ "unimplemented") 
-
-let optHashAlg_prime_is_optHashAlg (ha:result hashAlg') : Tot (result hashAlg) =
-  match ha with
-  | Error(z) -> Error(z)
-  | Correct(h) -> Correct(h)
-
-let sigHashAlg_is_tuple_sig_hash (sha:sigHashAlg) : Tot (sigAlg * hashAlg) = 
-  match sha with | a,b -> a,b
-
-let rec list_sigHashAlg_is_list_tuple_sig_hash (lsha:list sigHashAlg) : Tot (list (sigAlg * hashAlg)) =
-  match lsha with
-  | [] -> []
-  | hd::tl -> (sigHashAlg_is_tuple_sig_hash hd)::(list_sigHashAlg_is_list_tuple_sig_hash tl)
-
-val verify_signature : chain -> pv:protocolVersion -> role -> csr:option bytes{is_None csr <==> pv = TLS_1p3} -> sigAlg -> option (list sigHashAlg) -> tbs:bytes -> sigv:bytes -> ST bool (fun _ -> True) (fun _ _ _ -> True)
-let verify_signature c pv role nonces csa sigalgs tbs sigv =
-  if length sigv > 4 then
-   let (h, r) = split sigv 1 in
-   let (sa, sigv) = split r 1 in
-   begin
-   match vlsplit 2 sigv with
-   | Correct (sigv, eof) ->
-       let tbs =
-	 begin
-         match pv with
-         | TLS_1p3 ->
-           let pad = abytes (String.make 64 (Char.char_of_int 32)) in
-           let ctx = match role with
-             | Server -> "TLS 1.3, server CertificateVerify"
-             | Client -> "TLS 1.3, client CertificateVerify" in
-           pad @| (abytes ctx) @| (abyte 0z) @| tbs
-         | _ -> (Some.v nonces) @| tbs
-	 end
-       in
-       begin
-	 match (length eof, parseSigAlg sa, optHashAlg_prime_is_optHashAlg(parseHashAlg h)) with
-         | 0, Correct sa, Correct (Hash h) ->
-           let algs : list sigHashAlg =
-	     begin
-	     match sigalgs with
-             | Some l -> l
-             | None -> [(csa, Hash CoreCrypto.SHA1)]
-	     end in
-             if List.Tot.existsb (fun (xs,xh)->(xs=sa && xh=Hash h)) (list_sigHashAlg_is_list_tuple_sig_hash algs) then
-	       begin
-	       match get_chain_public_signing_key c sa with
-	       | Correct pk ->
-	         let a = Signature.Use (fun _ -> True) sa [Hash h] false false in
-	         let (|_,pk|) = endorse #a pk in
-	         Signature.verify (Hash h) pk tbs sigv
-	       | Error z -> false
-	       end
-             else false
-         | _ -> false
-	 end
-    | _ -> false
-    end
-  else false
-
-private val check_length: list bytes -> chain -> Tot (result chain)
+private val check_length: list bytes -> chain -> Tot (option chain)
 let rec check_length cs acc =
   match cs with
-  | [] -> Correct (List.Tot.rev acc)
+  | [] -> Some (List.Tot.rev acc)
   | c::cs' ->
     if length c < 16777216 then check_length cs' (c::acc)
-    else Error(AD_decode_error, perror __SOURCE_FILE__ __LINE__ "")
+    else None
 
-val lookup_server_chain: string -> string -> protocolVersion -> option sigAlg -> option (list sigHashAlg) -> Tot (result (chain * CoreCrypto.certkey))
-let lookup_server_chain pem key pv sa ext_sig =
-(** TODO
-  let sal =
-    if is_None sa then None
-    else
-      let sa = Some.v sa in
-      (match ext_sig with
-      | None ->
-        (match pv with
-        | TLS_1p3 -> Error(AD_missing_extension, perror __SOURCE_FILE__ __LINE__ "missing supported signature algorithm extension in a 1.3 signature-based ciphersuite") // 6.3.2.1 of TLS 1.3 requires sending the "missing extension" alert 
-        | _ -> Correct (Some (sa, Hash CoreCrypto.SHA1)))
-               // This doesn't comply with 7.4.1.4.1. of RFC5246
-               // which requires selecting RSASIG regardless of the CS's sigAlg
-               // (thus enabling the use of ECDHE_ECDSA with RSA cert if extension is omitted)
-      | Some al -> List.Tot.tryFind (fun (s,_)->s=sa) al) in
-*)
-  match CoreCrypto.cert_load_chain pem key with
-  | Some (csk, chain) -> (
-      match check_length chain [] with
-      | Correct chain -> Correct (chain, csk)
-      | Error z -> Error z)
+// TODO: we could retrieve sa from the subjectPublicKey field of
+// the end certificate. We could also honor any hash algorithm
+// specified in the params, if present.
+val lookup_chain: pemfile:string -> Tot (result chain)
+let lookup_chain pemfile =
+  match CoreCrypto.load_chain pemfile with
+  | Some chain ->
+    begin
+    match check_length chain [] with
+    | Some chain -> Correct chain
+    | None -> Error(AD_no_certificate, perror __SOURCE_FILE__ __LINE__ "cannot find suitable server certificate")
+    end
   | None -> Error(AD_no_certificate, perror __SOURCE_FILE__ __LINE__ "cannot find suitable server certificate")
-
-val sign: pv:protocolVersion -> role -> csr:option bytes{is_None csr <==> pv = TLS_1p3} -> CoreCrypto.certkey -> sigHashAlg -> bytes -> Tot (result bytes)
-let sign pv role csr csk sha tbs =
-  let (sa, ha) = sha in
-  let Hash h = ha in
-  let hab, sab = hashAlgBytes ha, sigAlgBytes sa in
-  let tbs = match pv with
-    | TLS_1p3 ->
-      let pad = abytes (String.make 64 (Char.char_of_int 32)) in
-      let ctx = (match role with
-        | Server -> "TLS 1.3, server CertificateVerify"
-        | Client -> "TLS 1.3, client CertificateVerify") in
-      pad @| (abytes ctx) @| (abyte 0z) @| tbs
-    | _ -> (Some.v csr) @| tbs in
-  match CoreCrypto.cert_sign csk sa h tbs with
-  | Some sigv -> (
-      if length sigv >= 2 && length sigv < 65536 then (
-	lemma_repr_bytes_values (length sigv);
-	Correct (hab @| sab @| (vlbytes 2 sigv))
-	)
-      else Error(AD_decode_error, perror __SOURCE_FILE__ __LINE__ "")
-      )
-  | None -> Error(AD_internal_error, perror __SOURCE_FILE__ __LINE__ "failed to sign")
-
-//let certificate_sign: chain -> 
-
-(*
-type sign_cert = option (chain * Sig.alg * Sig.skey)
-type enc_cert  = option (chain * RSAKey.sk)
-
-abstract val for_signing : list Sig.alg -> hint -> list Sig.alg -> sign_cert
-let for_signing l h l2 = failwith "Not implemented"
-
-abstract val for_key_encryption : list Sig.alg -> hint -> enc_cert
-let for_key_encryption l h = failwith "Not implemented"
-
-abstract val get_public_signing_key : cert -> Sig.alg -> result Sig.pkey
-let get_public_signing_key c a = failwith "Not implemented"
-
-abstract val get_public_encryption_key : cert -> result RSAKey.pk
-let get_public_encryption_key c = failwith "Not implemented"
-
-abstract val get_chain_public_signing_key : chain -> Sig.alg -> result Sig.pkey
-let get_chain_public_signing_key c a = failwith "Not implemented"
-
-abstract val get_chain_public_encryption_key : chain -> result RSAKey.pk
-let get_chain_public_encryption_key c = failwith "Not implemented"
-
-abstract val is_chain_for_signing : chain -> bool
-let is_chain_for_signing c = failwith "Not implemented"
-
-abstract val is_chain_for_key_encryption : chain -> bool
-let is_chain_for_key_encryption c = failwith "Not implemented"
-
-abstract val get_hint : chain -> option hint
-let get_hint c = failwith "Not implemented"
-
-abstract val validate_cert_chain : list Sig.alg  -> chain -> bool
-let validate_cert_chain l c = failwith "Not implemented"
-*)
