src/tls/Handshake.fst
@@ -1,9 +1,6 @@
-﻿(* Copyright (C) 2012--2015 Microsoft Research and INRIA *)
-
-#light "off"
-
-(* Handshake protocol messages *)
+﻿(* Handshake protocol messages *)
 module Handshake
+
 open TLSExtensions //the other opens are in the .fsti
 open CoreCrypto
 open HSCrypto
@@ -13,24 +10,23 @@ let hsId h = noId // Placeholder
 
 (* Negotiation: HELLO sub-module *)
 
-let ri = (cVerifyData * sVerifyData) 
-
+let ri = (cVerifyData * sVerifyData)
 
 
 let prepareClientHello cfg ks log ri sido =
   let cr = KeySchedule.ks_client_random ks in
-  let kp = 
+  let kp =
      (match cfg.maxVer with
-      | TLS_1p3 -> 
-         let gxl = KeySchedule.ks_client_13_init_1rtt ks cfg.namedGroups in 
+      | TLS_1p3 ->
+         let gxl = KeySchedule.ks_client_13_init_1rtt ks cfg.namedGroups in
 	 Some (ClientKeyShare gxl)
-      | _ -> 
-      	 let _ = KeySchedule.ks_client_init_12 ks in 
+      | _ ->
+      	 let _ = KeySchedule.ks_client_init_12 ks in
 	 None) in
   let sid = (match sido with | None -> empty_bytes | Some x -> x) in
   let ci = initConnection Client cr in
   let ext = prepareExtensions cfg ci ri kp in
-  let ch = 
+  let ch =
   {ch_protocol_version = cfg.maxVer;
    ch_client_random = cr;
    ch_sessionID = sid;
@@ -76,14 +72,14 @@ val getCachedSession: cfg:config -> ch:ch -> ST (option session)
 let getCachedSession cfg cg = None
 
 val negotiateGroupKeyShare: cfg:config -> protocolVersion -> kexAlg -> exts:option (list extension) -> Tot (result (namedGroup * option bytes))
-let rec negotiateGroupKeyShare cfg pv kex exts = 
+let rec negotiateGroupKeyShare cfg pv kex exts =
     match pv,kex,exts with
     | TLS_1p3, Kex_ECDHE, Some (E_keyShare (ClientKeyShare ((gn,gxb)::_)) :: _) ->
       Correct (gn,Some gxb)
     | TLS_1p3,_, Some (h::t) -> negotiateGroupKeyShare cfg pv kex (Some t)
-    | TLS_1p2, Kex_ECDHE, _ -> Correct (SEC CoreCrypto.ECC_P256, None) 
+    | TLS_1p2, Kex_ECDHE, _ -> Correct (SEC CoreCrypto.ECC_P256, None)
     | _ -> Error(AD_decode_error, "no supported group or key share extension found")
-    
+
 
 // FIXME: TLS1.3
 let prepareServerHello cfg ks log ri (ClientHello ch,_) =
@@ -97,9 +93,9 @@ let prepareServerHello cfg ks log ri (ClientHello ch,_) =
     | Error(z) -> Error(z)
     | Correct(gn,gxo) ->
   let srand = KeySchedule.ks_server_random ks in
-  let ksl = 
+  let ksl =
     (match pv,gxo with
-     | TLS_1p3,Some gxb -> 
+     | TLS_1p3,Some gxb ->
        let gyb = KeySchedule.ks_server_13_1rtt_init ks ch.ch_client_random cs gn gxb in
        (Some (ServerKeyShare (gn,gyb)))
     | _ -> None) in
@@ -110,14 +106,14 @@ let prepareServerHello cfg ks log ri (ClientHello ch,_) =
     let comp = match ch.ch_compressions with
       | [] -> None
       | _ -> Some NullCompression in
-    let sh = 
+    let sh =
       {sh_protocol_version = pv;
        sh_sessionID = Some sid;
        sh_server_random = srand;
        sh_cipher_suite = cs;
        sh_compression = comp;
        sh_extensions = sext} in
-    let nego = 
+    let nego =
       {n_client_random = ch.ch_client_random;
        n_server_random = srand;
        n_sessionID = Some sid;
@@ -150,7 +146,7 @@ let isSentinelRandomValue c_pv s_pv s_random =
 val acceptableVersion: config -> ch -> protocolVersion -> TLSInfo.random -> Tot bool
 let acceptableVersion cfg ch s_pv s_random =
   match negotiateVersion cfg ch.ch_protocol_version with
-  | Correct c_pv -> 
+  | Correct c_pv ->
     gte_pv c_pv s_pv && gte_pv s_pv cfg.minVer &&
     not (isSentinelRandomValue c_pv s_pv s_random)
   | Error _ ->
@@ -168,10 +164,10 @@ let acceptableCipherSuite cfg ch s_pv s_cs =
   List.Tot.existsb (fun x -> x = s_cs) ch.ch_cipher_suites &&
   List.Tot.existsb (fun x -> x = s_cs) cfg.ciphersuites &&
   not (isAnonCipherSuite s_cs) || cfg.allowAnonCipherSuite
-  
+
 let processServerHello cfg ks log ri ch (ServerHello sh,_) =
   let _ = log @@ (ServerHello sh) in
-  // Assuming no resumption; TODO: add it 
+  // Assuming no resumption; TODO: add it
   if not (acceptableVersion cfg ch sh.sh_protocol_version sh.sh_server_random) then
     Error(AD_illegal_parameter, perror __SOURCE_FILE__ __LINE__ "Protocol version negotiation")
   else  if not (acceptableCipherSuite cfg ch sh.sh_protocol_version sh.sh_cipher_suite) then
@@ -180,10 +176,10 @@ let processServerHello cfg ks log ri ch (ServerHello sh,_) =
   let resume = false in
   match negotiateClientExtensions sh.sh_protocol_version cfg ch.ch_extensions sh.sh_extensions sh.sh_cipher_suite ri resume with
     | Error z -> Error z
-    | Correct next -> 
+    | Correct next ->
         match sh.sh_cipher_suite with
 	| CipherSuite kex sa ae ->
-        let o_nego = 
+        let o_nego =
           {n_client_random = ch.ch_client_random;
            n_server_random = sh.sh_server_random;
            n_sessionID = sh.sh_sessionID;
@@ -198,8 +194,8 @@ let processServerHello cfg ks log ri ch (ServerHello sh,_) =
            n_extensions = next;
            n_resume = false } in
 	   (match sh.sh_protocol_version, kex, next.ne_keyShare with
-	    | TLS_1p3, Kex_DHE, Some (gn,gyb) 
-	    | TLS_1p3, Kex_ECDHE, Some (gn,gyb) -> 
+	    | TLS_1p3, Kex_DHE, Some (gn,gyb)
+	    | TLS_1p3, Kex_ECDHE, Some (gn,gyb) ->
 	      	   let lb = HandshakeLog.getHash log in
 	           let keys = KeySchedule.ks_client_13_1rtt ks o_nego.n_cipher_suite (gn, gyb) lb in
 	      	   Correct (o_nego,Some keys)
@@ -209,7 +205,7 @@ let processServerHello cfg ks log ri ch (ServerHello sh,_) =
 
 (* Handshake API: TYPES, taken from FSTI *)
 
-type clientState = 
+type clientState =
   | C_Idle: option ri -> clientState
   | C_HelloSent: option ri -> ch -> clientState
   | C_HelloReceived: nego -> clientState
@@ -218,7 +214,7 @@ type clientState =
   | C_CCSReceived: nego -> cVerifyData -> clientState
   | C_Error: error -> clientState
 
-type serverState = 
+type serverState =
      | S_Idle : option ri -> serverState
      | S_HelloSent : nego -> serverState
      | S_HelloDone : nego -> serverState
@@ -229,7 +225,7 @@ type serverState =
      | S_ZeroRTTReceived : nego -> serverState
      | S_Error: error -> serverState
 
-  
+
 type hs_msg_bufs = {
      hs_incoming_parsed : list (hs_msg * bytes);
      hs_incoming: bytes;
@@ -242,10 +238,10 @@ let hs_msg_bufs_init() = {
      hs_outgoing = empty_bytes;
 }
 
-type role_state = 
+type role_state =
     | C of clientState
     | S of serverState
-     
+
 type handshake_state' (r:role) =
      {
        hs_state: role_state;
@@ -284,7 +280,7 @@ let handshake_state_init cfg (r:role) (reg:rid) =
 
 //Defined in the .fsti
 //type handshake
-//type epoch 
+//type epoch
 //type epochs
 //type hs
 //type outgoing
@@ -300,15 +296,15 @@ assume val deriveEpoch: (r:rid) -> (n:TLSInfo.random) -> session -> ST (epoch r 
 val client_send_client_hello: hs -> ST unit
   (requires (fun h -> True))
   (ensures (fun h0 i h1 -> True))
-let client_send_client_hello (HS #r0 r res cfg id lgref hsref) = 
+let client_send_client_hello (HS #r0 r res cfg id lgref hsref) =
   match (!hsref).hs_state with
-  | C(C_Idle ri) -> 
+  | C(C_Idle ri) ->
     let (ClientHello ch,chb) = prepareClientHello cfg (!hsref).hs_ks (!hsref).hs_log ri None in
-    hsref := {!hsref with 
+    hsref := {!hsref with
             hs_buffers = {(!hsref).hs_buffers with hs_outgoing = chb};
 	    hs_state = C(C_HelloSent ri ch)}
-  
-	    
+
+
 val client_handle_server_hello: hs -> list (hs_msg * bytes) -> ST incoming
   (requires (fun h -> True))
   (ensures (fun h0 i h1 -> True))
@@ -317,87 +313,151 @@ let client_handle_server_hello (HS #r0 r res cfg id lgref hsref) msgs =
   | C(C_HelloSent ri ch),[(ServerHello(sh),l)] ->
    (match (processServerHello cfg (!hsref).hs_ks (!hsref).hs_log ri ch (ServerHello sh,l)) with
     | Error z -> InError z
-    | Correct (n,k) -> 
+    | Correct (n,k) ->
       hsref := {!hsref with
 	       hs_nego = Some n;
 	       hs_state = C(C_HelloReceived n)};
       InAck)
 
 
+let optHashAlg_prime_is_optHashAlg: result hashAlg' -> Tot (result hashAlg) =
+  function
+  | Error z -> Error z
+  | Correct h -> Correct h
+
+let sigHashAlg_is_tuple_sig_hash: sigHashAlg -> Tot (sigAlg * hashAlg) =
+  function | a,b -> a,b
+
+let rec list_sigHashAlg_is_list_tuple_sig_hash: list sigHashAlg -> Tot (list (sigAlg * hashAlg)) =
+  function
+  | [] -> []
+  | hd::tl -> (sigHashAlg_is_tuple_sig_hash hd) :: (list_sigHashAlg_is_list_tuple_sig_hash tl)
+
+val to_be_signed: pv:protocolVersion -> role -> csr:option bytes{is_None csr <==> pv = TLS_1p3} -> bytes -> Tot bytes
+let to_be_signed pv role csr tbs =
+  match pv, csr with
+  | TLS_1p3, None ->
+    let pad = abytes (String.make 64 (Char.char_of_int 32)) in
+    let ctx =
+      match role with
+      | Server -> "TLS 1.3, server CertificateVerify"
+      | Client -> "TLS 1.3, client CertificateVerify"
+    in
+    pad @| (abytes ctx) @| (abyte 0z) @| tbs
+  | _, Some csr -> csr @| tbs
+
+val sigHashAlg_of_ske: bytes -> Tot (option (sigHashAlg * bytes))
+let sigHashAlg_of_ske signature =
+  if length signature > 4 then
+   let h, sa, sigv = split2 signature 1 1 in
+   match vlsplit 2 sigv with
+   | Correct (sigv, eof) ->
+     begin
+     match length eof, parseSigAlg sa, optHashAlg_prime_is_optHashAlg (parseHashAlg h) with
+     | 0, Correct sa, Correct (Hash h) -> Some ((sa,Hash h), sigv)
+     | _, _, _ -> None
+     end
+   | Error _ -> None
+  else None
+
+
 let processServerHelloDone cfg n ks log msgs opt_msgs =
   match msgs with
-  | [(Certificate(c),_); (ServerKeyExchange(ske),_); (ServerHelloDone,_)] when 
-     (n.n_protocol_version <> TLS_1p3 && is_Some n.n_sigAlg &&
-      (n.n_kexAlg = Kex_DHE || n.n_kexAlg = Kex_ECDHE)) -> 
-     // Validate the server certificate chain before doing anything with other message
-     // TODO add check for n.n_extensions.ne_signature_algorithms
-     if (not cfg.check_peer_certificate) || Cert.validate_chain c.crt_chain n.n_sigAlg cfg.peer_name cfg.ca_file then
+  | [(Certificate(c),_); (ServerKeyExchange(ske),_); (ServerHelloDone,_)]
+    when (n.n_protocol_version <> TLS_1p3 && is_Some n.n_sigAlg &&
+      (n.n_kexAlg = Kex_DHE || n.n_kexAlg = Kex_ECDHE)) ->
+     if (not cfg.check_peer_certificate) || Cert.validate_chain c.crt_chain true cfg.peer_name cfg.ca_file then
        let ske_tbs = kex_s_to_bytes ske.ske_kex_s in
        let ske_sig = ske.ske_sig in
-       let cs_sigalg = Some.v n.n_sigAlg in
-       let csr = (n.n_client_random @| n.n_server_random) in
-       let ems = n.n_extensions.ne_extended_ms in
-
-       let valid = Cert.verify_signature c.crt_chain n.n_protocol_version Server (Some csr) 
-          cs_sigalg n.n_extensions.ne_signature_algorithms ske_tbs ske_sig in
-       let _ = IO.debug_print_string("Signature validation status = "^(if valid then "OK" else "FAIL")^"\n") in
-       if valid then
-         (match ske.ske_kex_s with
-         | KEX_S_DHE gy ->
-           let gx = KeySchedule.ks_client_12_full_dh ks n.n_server_random n.n_protocol_version 
-	            n.n_cipher_suite n.n_extensions.ne_extended_ms gy in 
-           let cke = {cke_kex_c = kex_c_of_dh_key gx} in
-            (match opt_msgs with 
-            | [] -> 
-	      let _ = log @@ Certificate(c) in
-	      let _ = log @@ ServerKeyExchange(ske) in
-	      let _ = log @@ ServerHelloDone in
-	      let b = log @@ ClientKeyExchange cke in
-	      let lb = HandshakeLog.getBytes log in
-	      if ems then KeySchedule.ks_client_12_set_session_hash ks lb;
-	      Correct [(ClientKeyExchange cke,b)]
-            | [(CertificateRequest(cr),_)] ->
-              let cc = {crt_chain = []} in // TODO
-	      let _ = log @@ Certificate(c) in
-	      let _ = log @@ ServerKeyExchange(ske) in
-	      let _ = log @@ CertificateRequest(cr) in
-	      let _ = log @@ ServerHelloDone in
-	      let b1 = log @@ ClientKeyExchange cke in	
-	      let lb = HandshakeLog.getBytes log in
-	      if ems then KeySchedule.ks_client_12_set_session_hash ks lb;
-	      let b2 = log @@ Certificate(cc) in
-      	    Correct [ClientKeyExchange cke,b1; Certificate cc,b2])
-	  | _ -> Error (AD_handshake_failure, perror __SOURCE_FILE__ __LINE__ "only support ECDHE/DHE SKE")
-         )
-       // Signature verification failed
-       else Error (AD_handshake_failure, perror __SOURCE_FILE__ __LINE__ "failed to check SKE signature")
-     // Certificate validation failed
-     else Error (AD_certificate_unknown_fatal, perror __SOURCE_FILE__ __LINE__ "Certificate validation failure") 
-
+       let Some cs_sigalg = n.n_sigAlg in
+       let sigalgs = n.n_extensions.ne_signature_algorithms in
+       begin
+       match sigHashAlg_of_ske ske_sig with
+       | Some ((sa,h),sigv) ->
+         let algs: list sigHashAlg =
+           match sigalgs with
+           | Some l -> l
+           | None -> [(cs_sigalg, Hash CoreCrypto.SHA1)]
+         in
+         if List.Tot.existsb (fun (xs,xh) -> (xs = sa && xh = h))
+	      algs then
+           begin
+	   let a = Signature.Use (fun _ -> True) sa [h] false false in
+           let csr = (n.n_client_random @| n.n_server_random) in
+           let ems = n.n_extensions.ne_extended_ms in
+           let tbs = to_be_signed n.n_protocol_version Server (Some csr) ske_tbs in
+           match Signature.get_chain_public_key #a c.crt_chain with
+           | Some pk ->
+	     let valid = Signature.verify #a h pk tbs sigv in
+	     //let _ = IO.debug_print_string("tbs = " ^ (Platform.Bytes.print_bytes tbs) ^ "\n") in
+	     let _ = IO.debug_print_string("Signature validation status = " ^ (if valid then "OK" else "FAIL") ^ "\n") in
+	     if valid then
+	       begin
+               match ske.ske_kex_s with
+               | KEX_S_DHE gy ->
+                 let gx = KeySchedule.ks_client_12_full_dh ks n.n_server_random n.n_protocol_version n.n_cipher_suite n.n_extensions.ne_extended_ms gy in
+                 let cke = {cke_kex_c = kex_c_of_dh_key gx} in
+                   begin
+	           match opt_msgs with
+                   | [] ->
+	             let _ = log @@ Certificate(c) in
+	             let _ = log @@ ServerKeyExchange(ske) in
+	             let _ = log @@ ServerHelloDone in
+	             let b = log @@ ClientKeyExchange cke in
+	             let lb = HandshakeLog.getBytes log in
+	             if ems then KeySchedule.ks_client_12_set_session_hash ks lb;
+	             Correct [(ClientKeyExchange cke,b)]
+                   | [(CertificateRequest(cr),_)] ->
+                     let cc = {crt_chain = []} in // TODO
+	             let _ = log @@ Certificate(c) in
+	             let _ = log @@ ServerKeyExchange(ske) in
+	             let _ = log @@ CertificateRequest(cr) in
+	             let _ = log @@ ServerHelloDone in
+	             let b1 = log @@ ClientKeyExchange cke in
+	             let lb = HandshakeLog.getBytes log in
+	             if ems then KeySchedule.ks_client_12_set_session_hash ks lb;
+	             let b2 = log @@ Certificate(cc) in
+      	             Correct [ClientKeyExchange cke,b1; Certificate cc,b2]
+		   | _ ->
+		     Error (AD_handshake_failure, perror __SOURCE_FILE__ __LINE__ "only support ECDHE/DHE SKE")
+	           end
+	       | _ -> Error (AD_handshake_failure, perror __SOURCE_FILE__ __LINE__ "only support ECDHE/DHE SKE")
+               end
+             // Signature verification failed
+             else Error (AD_handshake_failure, perror __SOURCE_FILE__ __LINE__ "failed to check SKE signature")
+	     // Algorithm negotiation failed
+	   | None -> Error (AD_handshake_failure, perror __SOURCE_FILE__ __LINE__ "failed to get public key from chain")
+	   end
+         // Certificate validation failed
+         else Error (AD_handshake_failure, perror __SOURCE_FILE__ __LINE__ "Signature algorithm negotiation failed")
+       | None -> Error (AD_decode_error, perror __SOURCE_FILE__ __LINE__ "Failed to parse SKE message")
+       end
+     else Error (AD_certificate_unknown_fatal, perror __SOURCE_FILE__ __LINE__ "Certificate validation failure")
+  | _ -> Error (AD_handshake_failure, perror __SOURCE_FILE__ __LINE__ "Unexpected message")
 
 val client_handle_server_hello_done: hs -> list (hs_msg * bytes) -> list (hs_msg * bytes) -> ST incoming
   (requires (fun h -> True))
   (ensures (fun h0 i h1 -> True))
 let client_handle_server_hello_done (HS #r0 r res cfg id lgref hsref) msgs opt_msgs =
   match (!hsref).hs_state with
-  | C(C_HelloReceived n) when 
+  | C(C_HelloReceived n) when
      (n.n_protocol_version <> TLS_1p3 && is_Some n.n_sigAlg &&
-      (n.n_kexAlg = Kex_DHE || n.n_kexAlg = Kex_ECDHE)) -> 
+      (n.n_kexAlg = Kex_DHE || n.n_kexAlg = Kex_ECDHE)) ->
      (match processServerHelloDone cfg n (!hsref).hs_ks (!hsref).hs_log msgs opt_msgs with
       | Correct [(ClientKeyExchange(cke),b1)] ->
-             hsref := {!hsref with 
+             hsref := {!hsref with
                 hs_buffers = {(!hsref).hs_buffers with hs_outgoing = b1};
                 hs_state = C(C_OutCCS n)};
               InAck
       | Correct [(ClientKeyExchange(cke),b1);(Certificate(cc),b2)] ->
-             hsref := {!hsref with 
+             hsref := {!hsref with
                 hs_buffers = {(!hsref).hs_buffers with hs_outgoing = b1 @| b2};
                 hs_state = C(C_OutCCS n)};
               InAck
       | Error (x,y) -> InError(x,y))
    | _ -> InError (AD_handshake_failure, perror __SOURCE_FILE__ __LINE__ "unexpected state")
 
-let prepareClientFinished ks log = 
+let prepareClientFinished ks log =
     let lb = HandshakeLog.getBytes log in
     let fin = {fin_vd = KeySchedule.ks_client_12_client_verify_data ks lb} in
     let finb = log @@ (Finished fin) in
@@ -411,11 +471,11 @@ let client_send_client_finished (HS #r0 r res cfg id lgref hsref) =
   match hs.hs_state with
   | C(C_OutCCS n) ->
      let (Finished fin,finb) = prepareClientFinished (!hsref).hs_ks (!hsref).hs_log in
-     hsref := {!hsref with 
+     hsref := {!hsref with
             hs_buffers = {(!hsref).hs_buffers with hs_outgoing = finb};
 	    hs_state = C(C_FinishedSent n fin.fin_vd)}
-  
-  
+
+
 val client_handle_server_ccs: hs -> list (hs_msg * bytes) -> ST incoming
   (requires (fun h -> True))
   (ensures (fun h0 i h1 -> True))
@@ -432,7 +492,7 @@ let processServerFinished ks log (m,l) =
    | Finished(f) ->
      let lb = HandshakeLog.getBytes log in
      let svd = KeySchedule.ks_client_12_server_verify_data ks lb in
-     if (equalBytes svd f.fin_vd) then 
+     if (equalBytes svd f.fin_vd) then
      	let _ = log @@ (Finished(f)) in
 	Correct svd
      else Error (AD_decode_error, "Finished MAC did not verify")
@@ -446,53 +506,70 @@ let client_handle_server_finished (HS #r0 r res cfg id lgref hsref) msgs =
   | C(C_CCSReceived n vd), [(Finished(f),l)] ->
    (match processServerFinished (!hsref).hs_ks (!hsref).hs_log (Finished f,l) with
     | Error z -> InError z
-    | Correct svd -> 
+    | Correct svd ->
        hsref := {!hsref with
   		 hs_state = C(C_Idle (Some (vd,svd)))};
        InAck)
-    
+
 
 let processServerFinished_13 cfg n ks log msgs =
-   let rem,creq = 
+   let rem,creq =
      match msgs with
-     | (EncryptedExtensions ee,_) :: (CertificateRequest cr,_) :: rem ->         
-       let _ = log @@ EncryptedExtensions(ee) in 
-       let _ = log @@ CertificateRequest(cr) in 
+     | (EncryptedExtensions ee,_) :: (CertificateRequest cr,_) :: rem ->
+       let _ = log @@ EncryptedExtensions(ee) in
+       let _ = log @@ CertificateRequest(cr) in
        rem,true
-     | (EncryptedExtensions ee,_) :: rem ->         
-       let _ = log @@ EncryptedExtensions(ee) in 
+     | (EncryptedExtensions ee,_) :: rem ->
+       let _ = log @@ EncryptedExtensions(ee) in
        rem,false in
     match rem with
-    | [(Certificate c,_); (CertificateVerify cv,_); (Finished f,_)] 
-     when (is_Some n.n_sigAlg && (n.n_kexAlg = Kex_DHE || n.n_kexAlg = Kex_ECDHE)) -> 
-     if Cert.validate_chain c.crt_chain n.n_sigAlg cfg.peer_name cfg.ca_file then
-     let _ = log @@ Certificate(c) in
-     let lb = HandshakeLog.getHash log in
-     let cs_sigalg = Some.v n.n_sigAlg in
-     let valid = Cert.verify_signature c.crt_chain n.n_protocol_version Server None
-          cs_sigalg n.n_extensions.ne_signature_algorithms lb cv.cv_sig in
-     let _ = IO.debug_print_string("Signature validation status = "^(if valid then "OK" else "FAIL")^"\n") in
-     if valid then
-     let _ = log @@ CertificateVerify(cv) in
-     let lb = HandshakeLog.getHash log in
-     let svd = KeySchedule.ks_client_13_1rtt_server_finished ks lb in
-     if (equalBytes svd f.fin_vd) then 
-     	let _ = log @@ (Finished(f)) in
-	let lb = HandshakeLog.getHash log in
-	let (cvd,keys) = KeySchedule.ks_client_13_1rtt_client_finished ks lb in	
-	let cfin = {fin_vd = cvd} in
-	if creq then 
-	   let cc = {crt_chain = []} in 
-	   let ccb = log @@ Certificate(cc) in
-	   let finb = log @@ Finished(cfin) in
-	   Correct ([(Certificate(cc),ccb);(Finished(cfin),finb)],svd,keys)
-	else
-	   let finb = log @@ Finished(cfin) in
-	   Correct ([(Finished(cfin),finb)],svd,keys)
-     else Error (AD_decode_error, "Finished MAC did not verify")
-     else Error (AD_decode_error, "Certificate signature did not verify")
+    | [(Certificate c,_); (CertificateVerify cv,_); (Finished f,_)]
+     when (is_Some n.n_sigAlg && (n.n_kexAlg = Kex_DHE || n.n_kexAlg = Kex_ECDHE)) ->
+     if (not cfg.check_peer_certificate) || Cert.validate_chain c.crt_chain true cfg.peer_name cfg.ca_file then
+       let _ = log @@ Certificate(c) in
+       let lb = HandshakeLog.getHash log in
+       let Some cs_sigalg = n.n_sigAlg in
+       let Some algs = n.n_extensions.ne_signature_algorithms in
+       //let _ = IO.debug_print_string("cv_sig = " ^ (Platform.Bytes.print_bytes cv.cv_sig) ^ "\n") in
+       begin
+       match sigHashAlg_of_ske cv.cv_sig with
+       | Some ((sa,h), sigv) ->
+         if List.Tot.existsb (fun (xs,xh) -> (xs = sa && xh = h))
+             (list_sigHashAlg_is_list_tuple_sig_hash algs) then
+           begin
+           let a = Signature.Use (fun _ -> True) sa [h] false false in
+           let tbs = to_be_signed n.n_protocol_version Server None lb in
+           match Signature.get_chain_public_key #a c.crt_chain with
+           | Some pk ->
+             let valid = Signature.verify h pk tbs sigv in
+             let _ = IO.debug_print_string("Signature validation status = " ^ (if valid then "OK" else "FAIL") ^ "\n") in
+             if valid then
+               let _ = log @@ CertificateVerify(cv) in
+               let lb = HandshakeLog.getHash log in
+               let svd = KeySchedule.ks_client_13_1rtt_server_finished ks lb in
+               if (equalBytes svd f.fin_vd) then
+		 let _ = log @@ (Finished(f)) in
+        	 let lb = HandshakeLog.getHash log in
+        	 let (cvd,keys) = KeySchedule.ks_client_13_1rtt_client_finished ks lb in
+        	 let cfin = {fin_vd = cvd} in
+        	 if creq then
+        	   let cc = {crt_chain = []} in
+        	   let ccb = log @@ Certificate(cc) in
+        	   let finb = log @@ Finished(cfin) in
+        	   Correct ([(Certificate(cc),ccb);(Finished(cfin),finb)],svd,keys)
+        	 else
+        	   let finb = log @@ Finished(cfin) in
+        	   Correct ([(Finished(cfin),finb)],svd,keys)
+               else Error (AD_decode_error, "Finished MAC did not verify")
+             else Error (AD_decode_error, "Certificate signature did not verify")
+	   | None -> Error (AD_decode_error, "Certificate was not valid")
+	   end
+         else Error (AD_handshake_failure, "Signature algorithm negotiation failed")
+       | None -> Error (AD_decode_error, "Failed to parse message")
+       end
      else Error (AD_decode_error, "Certificate was not valid")
    | _ -> Error (AD_decode_error, "Unexpected state")
+   
 
 val client_handle_server_finished_13: hs -> list (hs_msg * bytes) -> ST incoming
   (requires (fun h -> True))
@@ -502,17 +579,17 @@ let client_handle_server_finished_13 (HS #r0 r res cfg id lgref hsref) msgs =
   | C(C_CCSReceived n vd) ->
    (match processServerFinished_13 cfg n (!hsref).hs_ks (!hsref).hs_log msgs with
     | Error z -> InError z
-    | Correct ([(Finished(f),fb)],svd,keys) -> 
+    | Correct ([(Finished(f),fb)],svd,keys) ->
        hsref := {!hsref with
                  hs_buffers = {(!hsref).hs_buffers with hs_outgoing = fb};
   		 hs_state = C(C_Idle (Some (vd,svd)))};
        InAck
-    | Correct ([(Certificate c,cb);(Finished f,fb)],svd,keys) -> 
+    | Correct ([(Certificate c,cb);(Finished f,fb)],svd,keys) ->
        hsref := {!hsref with
                  hs_buffers = {(!hsref).hs_buffers with hs_outgoing = cb @| fb};
   		 hs_state = C(C_Idle (Some (vd,svd)))};
        InAck)
-    
+
 
 
 
@@ -530,60 +607,97 @@ let server_handle_client_hello (HS #r0 r res cfg id lgref hsref) msgs =
 	       hs_nego = Some n;
 	       hs_state = S(S_HelloSent n)};
        InAck)
-    
 
+(** TODO
+  let sal =
+    if is_None sa then None
+    else
+      let sa = Some.v sa in
+      (match ext_sig with
+      | None ->
+        (match pv with
+        | TLS_1p3 -> Error(AD_missing_extension, perror __SOURCE_FILE__ __LINE__ "missing supported signature algorithm extension in a 1.3 signature-based ciphersuite") // 6.3.2.1 of TLS 1.3 requires sending the "missing extension" alert
+        | _ -> Correct (Some (sa, Hash CoreCrypto.SHA1)))
+               // This doesn't comply with 7.4.1.4.1. of RFC5246
+               // which requires selecting RSASIG regardless of the CS's sigAlg
+               // (thus enabling the use of ECDHE_ECDSA with RSA cert if extension is omitted)
+      | Some al -> List.Tot.tryFind (fun (s,_)->s=sa) al) in
+*)
 val server_send_server_hello_done: hs -> ST unit
   (requires (fun h -> True))
   (ensures (fun h0 i h1 -> True))
 let server_send_server_hello_done (HS #r0 r res cfg id lgref hsref) =
   match (!hsref).hs_state with
-  | S(S_HelloSent n) 
+  | S(S_HelloSent n)
     when (n.n_protocol_version <> TLS_1p3 &&
 	 (n.n_kexAlg = Kex_DHE || n.n_kexAlg = Kex_ECDHE)) ->
-    (match Cert.lookup_server_chain cfg.cert_chain_file cfg.private_key_file n.n_protocol_version n.n_sigAlg n.n_extensions.ne_signature_algorithms with
-    | Correct (chain, csk) -> 
+    begin
+    match Cert.lookup_chain cfg.cert_chain_file with
+    | Correct chain ->
       let c = {crt_chain = chain} in
       let cb = certificateBytes n.n_protocol_version c in
       let gy = CommonDH.keygen CommonDH.default_group in
       let kex_s = KEX_S_DHE gy in
       let sv = kex_s_to_bytes kex_s in
-      let csr = n.n_client_random @| n.n_server_random in
-
-      // Signature agility (following the broken rules of 7.4.1.4.1. in RFC5246
       let Some sa = n.n_sigAlg in
-      let algs = match n.n_extensions.ne_signature_algorithms with
-        | None -> [sa,Hash CoreCrypto.SHA1] | Some l -> l in
-      let algs = List.Tot.filter (fun (s,_)->s=sa) algs in
-      let alg = match algs with | h::_ -> h | [] -> (sa, Hash CoreCrypto.SHA1) in
-      (match Cert.sign n.n_protocol_version Server (Some csr) csk alg sv with
-      | Correct signature -> 
-         let ske = {ske_kex_s = kex_s; ske_sig = signature} in
-         let skeb = serverKeyExchangeBytes ske in
-         let shd = serverHelloDoneBytes in
-         let nl = cb @| skeb @| shd in
-	    hsref := {!hsref with
-		 hs_buffers = {(!hsref).hs_buffers with hs_outgoing = nl};
-		 hs_log = (!hsref).hs_log (* @| nl *);
-		 hs_state = S(S_HelloDone n)}
-      | Error e -> 
-	  hsref := {!hsref with hs_state = S(S_Error e)})
-    | Error e ->
-        hsref := {!hsref with hs_state = S(S_Error e)})
+      let sigalgs = n.n_extensions.ne_signature_algorithms in
+      let algs =
+	match sigalgs with
+	| Some l -> l
+	| None -> [(sa,Hash CoreCrypto.SHA1)]
+      in
+      let algs = List.Tot.filter (fun (s,_) -> s = sa) algs in
+      let sa, ha =
+	match algs with
+	| sha::_ -> sha
+	| [] -> (sa, Hash CoreCrypto.SHA1)
+      in
+      let hab, sab = hashAlgBytes ha, sigAlgBytes sa in
+      let a = Signature.Use (fun _ -> True) sa [ha] false false in
+      let csr = n.n_client_random @| n.n_server_random in
+      let tbs = to_be_signed n.n_protocol_version Server (Some csr) sv in
+      begin
+      match Signature.lookup_key #a cfg.private_key_file with
+      | Some csk ->
+	let sigv = Signature.sign ha csk tbs in
+        if length sigv >= 2 && length sigv < 65536 then
+	  begin
+	  lemma_repr_bytes_values (length sigv);
+	  let signature = (hab @| sab @| (vlbytes 2 sigv)) in
+	  let ske = {ske_kex_s = kex_s; ske_sig = signature} in
+	  let skeb = serverKeyExchangeBytes ske in
+	  let shd = serverHelloDoneBytes in
+	  let nl = cb @| skeb @| shd in
+	  hsref := {!hsref with
+		    hs_buffers = {(!hsref).hs_buffers with hs_outgoing = nl};
+	      hs_log = (!hsref).hs_log (* @| nl *);
+	      hs_state = S(S_HelloDone n)}
+	  end
+	else
+	  let e = (AD_decode_error, perror __SOURCE_FILE__ __LINE__ "Signature length out of range") in
+	  hsref := {!hsref with hs_state = S(S_Error e)}
+      | None ->
+        let e = (AD_decode_error, perror __SOURCE_FILE__ __LINE__ "Failed to get chain public key") in
+	hsref := {!hsref with hs_state = S(S_Error e)}
+      end
+    | Error e -> hsref := {!hsref with hs_state = S(S_Error e)}
+    end
+
 
 assume val server_handle_client_ccs: hs -> list (hs_msg * bytes) -> list (hs_msg * bytes) -> ST incoming
   (requires (fun h -> True))
   (ensures (fun h0 i h1 -> True))
 
 (*
-let server_handle_client_ccs (HS #r0 r res cfg id lgref hsref)  msgs opt_msgs = 
+let server_handle_client_ccs (HS #r0 r res cfg id lgref hsref)  msgs opt_msgs =
   match (!hsref).hs_state, msgs with
-  | S(S_HelloDone n),[(ClientKeyExchange(cke),l)] when 
-     (n.n_protocol_version <> TLS_1p3 && 
+  | S(S_HelloDone n),[(ClientKeyExchange(cke),l)] when
+     (n.n_protocol_version <> TLS_1p3 &&
       (n.n_kexAlg = Kex_DHE || n.n_kexAlg = Kex_ECDHE)) ->
-      let pms = CommonDH.dh_initiator k 
+      let pms = CommonDH.dh_initiator k
 *)
 
-    
+
 assume val server_handle_client_finished: hs -> list (hs_msg * bytes) -> ST incoming
   (requires (fun h -> True))
   (ensures (fun h0 i h1 -> True))
@@ -618,12 +732,12 @@ val iT_old:  s:hs -> rw:rw -> ST int
   (requires (fun h -> True))
   (ensures (fun h0 i h1 -> True))
 let iT_old (HS r res cfg id l st) rw =
-  match rw with 
+  match rw with
   | Reader -> (!st).hs_reader
   | Writer -> (!st).hs_writer
 
 //val init: see .fsti
-let init r0 r cfg res = 
+let init r0 r cfg res =
     let id = Nonce.mkHelloRandom r r0 in //NS: should this really be Client?
     let lgref = MS.alloc_mref_seq r0 Seq.createEmpty in
     let hs = handshake_state_init cfg r r0 in
@@ -642,19 +756,19 @@ let request s c = Platform.Error.unexpected "request: not yet implemented"
 let invalidateSession hs = Platform.Error.unexpected "invalidateSession: not yet implemented"
 
 //val next_fragment: see .fsti
-let rec next_fragment hs = 
+let rec next_fragment hs =
     let (HS #r0 r res cfg id lgref hsref) = hs in
-    let pv,kex,res = 
-      (match (!hsref).hs_nego with 
+    let pv,kex,res =
+      (match (!hsref).hs_nego with
        | None -> None, None, None
        | Some n -> Some n.n_protocol_version, Some n.n_kexAlg, Some n.n_resume) in
     let b = (!hsref).hs_buffers.hs_outgoing in
     let l = length b in
     if (l > 0) then (
        hsref := {!hsref with hs_buffers = {(!hsref).hs_buffers with hs_outgoing = empty_bytes}};
-       OutSome (l,l) b) 
-    else 
-      (match (!hsref).hs_state with 
+       OutSome (l,l) b)
+    else
+      (match (!hsref).hs_state with
        | C (C_Error e) -> OutError e
        | S (S_Error e) -> OutError e
        | C (C_Idle ri) -> (client_send_client_hello hs; next_fragment hs)
@@ -670,42 +784,42 @@ let rec parseHandshakeMessages pv kex buf =
     match parseMessage buf with
     | Error z -> Error z
     | Correct(None) -> Correct (buf,[])
-    | Correct(Some (|rem,hstype,pl,to_log|)) ->   
+    | Correct(Some (|rem,hstype,pl,to_log|)) ->
       (match parseHandshakeMessage pv kex hstype pl with
-       | Error z -> Error z 
-       | Correct hsm -> 
+       | Error z -> Error z
+       | Correct hsm ->
              (match parseHandshakeMessages pv kex rem with
        	     | Error z -> Error z
        	     | Correct (r,hsl) -> Correct(r,(hsm,to_log)::hsl)))
 
 
 //val recv_fragment: see .fsti
-let recv_fragment hs (rg:Range.range) (rb:rbytes rg) = 
+let recv_fragment hs (rg:Range.range) (rb:rbytes rg) =
     let (HS #r0 r res cfg id lgref hsref) = hs in
     let b = (!hsref).hs_buffers.hs_incoming in
     let b = b @| rb in
-    let pv,kex,res = 
-      (match (!hsref).hs_nego with 
+    let pv,kex,res =
+      (match (!hsref).hs_nego with
        | None -> None, None, None
        | Some n -> Some n.n_protocol_version, Some n.n_kexAlg, Some n.n_resume) in
     match parseHandshakeMessages pv kex b with
     | Error z -> InError z
-    | Correct(r,hsl) -> 
+    | Correct(r,hsl) ->
        hsref := {!hsref with hs_buffers = {(!hsref).hs_buffers with hs_incoming = r; hs_incoming_parsed = hsl}};
-      (match (!hsref).hs_state,hsl with 
+      (match (!hsref).hs_state,hsl with
        | C (C_Idle ri), _ -> InError(AD_unexpected_message, "Client hasn't sent hello yet")
-       | C (C_HelloSent ri ch), (ServerHello(sh),l)::hsl 
-	 when (sh.sh_protocol_version <> TLS_1p3 || hsl = []) -> 
+       | C (C_HelloSent ri ch), (ServerHello(sh),l)::hsl
+	 when (sh.sh_protocol_version <> TLS_1p3 || hsl = []) ->
 	   hsref := {!hsref with hs_buffers = {(!hsref).hs_buffers with hs_incoming_parsed = hsl}};
 	   client_handle_server_hello hs [(ServerHello(sh),l)]
        | C (C_HelloReceived n), (Certificate(c),l)::
 			          (ServerKeyExchange(ske),l')::
 				  (ServerHelloDone,l'')::
-				  hsl 
+				  hsl
 	 when (is_Some pv && pv <> Some TLS_1p3 && res = Some false &&
 	       (kex = Some Kex_DHE || kex = Some Kex_ECDHE)) ->
 	   hsref := {!hsref with hs_buffers = {(!hsref).hs_buffers with hs_incoming_parsed = hsl}};
-			   client_handle_server_hello_done hs 
+			   client_handle_server_hello_done hs
 			   [(Certificate(c),l) ;
 			   (ServerKeyExchange(ske),l') ;
 			   (ServerHelloDone,l'')]
@@ -714,32 +828,32 @@ let recv_fragment hs (rg:Range.range) (rb:rbytes rg) =
 			          (ServerKeyExchange(ske),l')::
 			          (CertificateRequest(cr),l'')::
 				  (ServerHelloDone,l''')::
-				  hsl 
+				  hsl
 	 when (is_Some pv && pv <> Some TLS_1p3 && res = Some false &&
 	       (kex = Some Kex_DHE || kex = Some Kex_ECDHE)) ->
 	   hsref := {!hsref with hs_buffers = {(!hsref).hs_buffers with hs_incoming_parsed = hsl}};
-			   client_handle_server_hello_done hs 
+			   client_handle_server_hello_done hs
 			   [(Certificate(c),l) ;
 			   (ServerKeyExchange(ske),l') ;
-			   (ServerHelloDone,l''')] 
+			   (ServerHelloDone,l''')]
 			   [(CertificateRequest(cr),l'')]
 
-       
-       | C (C_CCSReceived n cv), (Finished(f),l)::hsl 
+
+       | C (C_CCSReceived n cv), (Finished(f),l)::hsl
        	 when (is_Some pv && pv <> Some TLS_1p3) ->
 	   hsref := {!hsref with hs_buffers = {(!hsref).hs_buffers with hs_incoming_parsed = hsl}};
-			   client_handle_server_finished hs 
+			   client_handle_server_finished hs
 			   [(Finished(f),l)]
 
        | C (C_HelloReceived n), (EncryptedExtensions(ee),l1)::
 			          (Certificate(c),l2)::
 			          (CertificateVerify(cv),l3)::
 				  (Finished(f),l4)::
-				  [] 
-	 when (is_Some pv && pv = Some TLS_1p3 && 
+				  []
+	 when (is_Some pv && pv = Some TLS_1p3 &&
 	       (kex = Some Kex_DHE || kex = Some Kex_ECDHE)) ->
 	   hsref := {!hsref with hs_buffers = {(!hsref).hs_buffers with hs_incoming_parsed = []}};
-			   client_handle_server_finished_13 hs 
+			   client_handle_server_finished_13 hs
 			   [(EncryptedExtensions(ee),l1);
 			   (Certificate(c),l2) ;
 			   (CertificateVerify(cv),l3) ;
@@ -749,37 +863,37 @@ let recv_fragment hs (rg:Range.range) (rb:rbytes rg) =
 			          (Certificate(c),l2)::
 			          (CertificateVerify(cv),l3)::
 				  (Finished(f),l4)::
-				  [] 
-	 when (is_Some pv && pv = Some TLS_1p3 && 
+				  []
+	 when (is_Some pv && pv = Some TLS_1p3 &&
 	       (kex = Some Kex_DHE || kex = Some Kex_ECDHE)) ->
 	   hsref := {!hsref with hs_buffers = {(!hsref).hs_buffers with hs_incoming_parsed = []}};
-			   client_handle_server_finished_13 hs 
+			   client_handle_server_finished_13 hs
 			   [(EncryptedExtensions(ee),l1);
 			   (CertificateRequest(cr),ll);
-			   (Certificate(c),l2) ;			   
+			   (Certificate(c),l2) ;
 			   (CertificateVerify(cv),l3) ;
 			   (Finished(f),l4)]
-			   
-       
-       | S (S_Idle ri), (ClientHello(ch),l)::hsl -> 
+
+
+       | S (S_Idle ri), (ClientHello(ch),l)::hsl ->
 	   hsref := {!hsref with hs_buffers = {(!hsref).hs_buffers with hs_incoming_parsed = hsl}};
 			   server_handle_client_hello hs
 			   [(ClientHello(ch),l)]
-       | S (S_CCSReceived s), (Finished(f),l)::hsl 
+       | S (S_CCSReceived s), (Finished(f),l)::hsl
          when (is_Some pv && pv <> Some TLS_1p3) ->
 	   hsref := {!hsref with hs_buffers = {(!hsref).hs_buffers with hs_incoming_parsed = hsl}};
 			   server_handle_client_finished hs
 			   [(Finished(f),l)]
 
        | S (S_FinishedSent s), (ClientKeyExchange(cke),l)::
-			       (Finished(f),l')::[]  
+			       (Finished(f),l')::[]
          when (is_Some pv && pv = Some TLS_1p3) ->
 	   hsref := {!hsref with hs_buffers = {(!hsref).hs_buffers with hs_incoming_parsed = []}};
 	   server_handle_client_finished_13 hs [(ClientKeyExchange(cke),l);(Finished(f),l')] []
 
        | S (S_FinishedSent s), (ClientKeyExchange(cke),l1)::
 			       (Certificate(c),l2)::
-			       (Finished(f),l3)::[]  
+			       (Finished(f),l3)::[]
          when (is_Some pv && pv = Some TLS_1p3 && c.crt_chain = []) ->
 	   hsref := {!hsref with hs_buffers = {(!hsref).hs_buffers with hs_incoming_parsed = []}};
 	   server_handle_client_finished_13 hs [(ClientKeyExchange(cke),l1);(Finished(f),l3)] [(Certificate(c),l2)]
@@ -787,7 +901,7 @@ let recv_fragment hs (rg:Range.range) (rb:rbytes rg) =
        | S (S_FinishedSent s), (ClientKeyExchange(cke),l1)::
 			       (Certificate(c),l2)::
 			       (CertificateVerify(cv),l3)::
-			       (Finished(f),l4)::[]  
+			       (Finished(f),l4)::[]
          when (is_Some pv && pv = Some TLS_1p3) ->
 	   hsref := {!hsref with hs_buffers = {(!hsref).hs_buffers with hs_incoming_parsed = []}};
 	   server_handle_client_finished_13 hs [(ClientKeyExchange(cke),l1);(Finished(f),l4)] [(Certificate(c),l2);(CertificateVerify(cv),l3)]
@@ -795,41 +909,41 @@ let recv_fragment hs (rg:Range.range) (rb:rbytes rg) =
        | C (C_Error e),_ -> InError e
        | S (S_Error e),_ -> InError e
        | _ , _ -> InAck)
-	   
 
-//val recv_ccs: see .fsti  // special case: CCS before 1p3  
-let recv_ccs hs = 
+
+//val recv_ccs: see .fsti  // special case: CCS before 1p3
+let recv_ccs hs =
     let (HS #r0 r res cfg id lgref hsref) = hs in
-    let pv,kex = 
-      (match (!hsref).hs_nego with 
+    let pv,kex =
+      (match (!hsref).hs_nego with
        | None -> None, None
        | Some n -> Some n.n_protocol_version, Some n.n_kexAlg) in
-    (match ((!hsref).hs_state,(!hsref).hs_buffers.hs_incoming_parsed) with 
-    | C (C_FinishedSent n cv), 
+    (match ((!hsref).hs_state,(!hsref).hs_buffers.hs_incoming_parsed) with
+    | C (C_FinishedSent n cv),
       (SessionTicket(st),l)::[] ->
        hsref := {!hsref with hs_buffers = {(!hsref).hs_buffers with hs_incoming_parsed = []}};
-       client_handle_server_ccs hs 
+       client_handle_server_ccs hs
         [(SessionTicket(st),l)]
-    | S (S_HelloDone n), 
-      (ClientKeyExchange(cke),l)::[] 
-      when (is_Some pv && pv <> Some TLS_1p3 && 
+    | S (S_HelloDone n),
+      (ClientKeyExchange(cke),l)::[]
+      when (is_Some pv && pv <> Some TLS_1p3 &&
             (kex = Some Kex_DHE || kex = Some Kex_ECDHE)) ->
       hsref := {!hsref with hs_buffers = {(!hsref).hs_buffers with hs_incoming_parsed = []}};
       server_handle_client_ccs hs
       [(ClientKeyExchange(cke),l)] []
-    | S (S_HelloDone n), 
+    | S (S_HelloDone n),
       (Certificate(c),l)::
-      (ClientKeyExchange(cke),l')::[] 
-      when (c.crt_chain = [] && is_Some pv && pv <> Some TLS_1p3 && 
+      (ClientKeyExchange(cke),l')::[]
+      when (c.crt_chain = [] && is_Some pv && pv <> Some TLS_1p3 &&
             (kex = Some Kex_DHE || kex = Some Kex_ECDHE)) ->
       hsref := {!hsref with hs_buffers = {(!hsref).hs_buffers with hs_incoming_parsed = []}};
       server_handle_client_ccs hs
       [(ClientKeyExchange(cke),l')] [(Certificate(c),l)]
-    | S (S_HelloDone n), 
+    | S (S_HelloDone n),
       (Certificate(c),l)::
       (ClientKeyExchange(cke),l')::
       (CertificateVerify(cv),l'')::[]
-      when (is_Some pv && pv <> Some TLS_1p3 && 
+      when (is_Some pv && pv <> Some TLS_1p3 &&
             (kex = Some Kex_DHE || kex = Some Kex_ECDHE)) ->
       hsref := {!hsref with hs_buffers = {(!hsref).hs_buffers with hs_incoming_parsed = []}};
       server_handle_client_ccs hs
